Logic/Modal/Basic/Soundness.lean
@@ -10,9 +10,9 @@ open Formula FrameConsequence
 
 variable {α β : Type u}
 
-theorem LogicK.sounds (Γ : Set (Formula α)) (hΓ : Γ = ∅) (p : Formula α) (f : Frame β) (d : Γ ⊢ᴴ(𝐊) p) : (Γ ⊨ᶠ[f] p) := by
+theorem LogicK.sounds' (Γ : Set (Formula α)) (hΓ : Γ = ∅) (p : Formula α) (f : Frame β) (d : Γ ⊢ᴴ(𝐊) p) : (Γ ⊨ᶠ[f] p) := by
   induction d <;> try {simp_all [satisfies];}
-  case wk _ _ _ hΓΔ _ ih =>
+  case wk ih =>
     simp_all only [def_emptyctx];
     exact ih (by aesop);
   case maxm Γ p ih =>
@@ -23,13 +23,13 @@ theorem LogicK.sounds (Γ : Set (Formula α)) (hΓ : Γ = ∅) (p : Formula α) 
     -- TODO: ここで排中律を仮定する必要は本当にあるのだろうか？
     by_cases (w ⊧ˢ[⟨f, V⟩] p) <;> simp_all [satisfies];
 
-lemma LogicK.weakSounds {p : Formula α} (f : Frame β) (h : ⊢ᴴ(𝐊) p) : (⊧ᶠ[f] p) := by
-  exact (show (⊢ᴴ(𝐊) p) → (⊧ᶠ[f] p) by simpa [Context.box_empty] using sounds (∅) rfl p f;) h;
+lemma LogicK.sounds {p : Formula α} (f : Frame β) (h : ⊢ᴴ(𝐊) p) : (⊧ᶠ[f] p) := by
+  exact (show (⊢ᴴ(𝐊) p) → (⊧ᶠ[f] p) by simpa [Context.box_empty] using sounds' ∅ rfl p f;) h;
 
 theorem LogicK.unprovable_bot {f : Frame β} : (⊬ᴴ(𝐊)! (⊥ : Formula α)) := by
   by_contra hC; simp at hC;
   suffices h : ⊧ᶠ[f] (⊥ : Formula α) by exact frames.bot_def h;
-  exact weakSounds f hC.some;
+  exact sounds f hC.some;
 
 end Hilbert
 
